Prove triple for durable stack's constructor

src/examples/durable_stack.v
@@ -12,7 +12,8 @@ From self.lang Require Import notation lang.
 From self.algebra Require Import view.
 From self.base Require Import primitive_laws class_instances.
 From self.high Require Import proofmode wpc_proofmode.
-From self.high Require Import dprop modalities resources crash_weakestpre weakestpre
+From self.high Require Import dprop abstract_state_instances modalities
+     resources crash_weakestpre weakestpre weakestpre_na weakestpre_at
      recovery_weakestpre lifted_modalities protocol no_buffer.
 
 (* TODO: Add the necessary fences in this example. *)
@@ -30,24 +31,28 @@ Definition mk_nil : expr :=
 
 Definition mk_stack : expr :=
   λ: <>,
-    let: "toHead" := ref_NA (mk_nil #()) in
-    "toHead".
+    let: "node" := ref_NA (InjL #()) in
+    WB "node" ;;
+    Fence ;;
+    ref_AT "node".
 
 (* Push takes as arguments the stack and the value to push to the stack. It
 returns unit once the element has been pushed.*)
 Definition push : expr :=
   λ: "toHead" "val",
-    (* let: "toVal" := ref_NA "val" in *)
     let: "toNext" := ref_NA #() in
     let: "newNode" := ref_NA (InjR ("val", "toNext")) in
+    WB "newNode" ;;
     (rec: "loop" <> :=
        let: "head" := ! "toHead" in
        "toNext" <- "head" ;;
+       WB "toNext" ;;
+       Fence ;;
        if: CAS "toHead" "head" "toNext"
        then #()
        else "loop" #()
     ) #().
-    
+
 (* Pop takes the stack and returns an option that contains the first value or
 none if the stack is empty. *)
 Definition pop : expr :=
@@ -65,75 +70,102 @@ Definition pop : expr :=
 (* Section constant. *)
 (*   Context `{nvmFixedG Σ}. *)
 
-(*   Definition constant_inv (dv : discreteState val) (v : val) (hG : nvmDeltaG Σ) : dProp Σ := *)
+(*   Definition constant_prot (dv : discreteState val) (v : val) (hG : nvmDeltaG Σ) : dProp Σ := *)
 (*     ⌜ dv.(get_discrete) = v ⌝. *)
 
-(*   Program Instance : LocationProtocol constant_inv := { bumper n := n }. *)
+(*   Program Instance : LocationProtocol constant_prot := { bumper n := n }. *)
 (*   Next Obligation. iIntros. by iApply post_crash_flush_pure. Qed. *)
 (*   Next Obligation. iIntros (???) "? !> //". Qed. *)
-  
+
 (* End constant. *)
 
 Section constant_alt.
+  Context `{Σ : gFunctors}.
   Context `{nvmFixedG Σ}.
 
-  Definition constant_inv (v1 : val) (_ : unit) (v2 : val) (hG : nvmDeltaG Σ) : dProp Σ :=
+  Definition constant_prot `{nvmFixedG Σ} (v1 : val) (_ : unit) (v2 : val) (hG : nvmDeltaG Σ) : dProp Σ :=
     ⌜ v1 = v2 ⌝.
 
-  Global Program Instance constant_inv_prot v : LocationProtocol (constant_inv v) := { bumper n := n }.
+  Global Program Instance constant_inv_prot v : LocationProtocol (constant_prot v) := { bumper n := n }.
   Next Obligation. iIntros. by iApply post_crash_flush_pure. Qed.
   Next Obligation. iIntros (????) "? !> //". Qed.
-  
+
 End constant_alt.
-  
+
 Section proof.
   Implicit Types (ℓ : loc).
   Context `{nvmFixedG Σ, nvmDeltaG Σ}.
+
+  Definition mapsto_na_flushed `{AbstractState ST} ℓ q (s : ST) : dProp Σ :=
+    ∃ (ss : list ST), ⌜ last ss = Some s ⌝ ∗ ℓ ↦{q} ss ∗ know_flush_lb ℓ s.
 
   (* We assume a per-element predicate. *)
   Context (ϕ : val → nvmDeltaG Σ → dProp Σ).
   (* The per-element predicate must be stable under the <PCF> modality and not
   use anything from the buffer. *)
-  Context `{∀ a b, IntoCrashFlush (ϕ a b) (ϕ a),
-            ∀ a b, IntoNoBuffer (ϕ a b) (ϕ a b)}.
+  Context `{∀ a nD, IntoCrashFlush (ϕ a nD) (ϕ a),
+            ∀ a nD, IntoNoBuffer (ϕ a nD) (ϕ a nD)}.
 
-  Definition node_inv (x : val) (ℓtoNext : loc) :=
+  (* There are four types of locations in the stack:
+     * toHead - AT - The pointer to the first element in the stack.
+     * toNext - NA - The pointer from a node to it's successor, this node is
+       changed up to a point after which it is never changed.
+     * node - NA - Points to the injection for each node. This pointer is never
+       changed.
+   *)
+
+  Definition toNext_prot : loc_pred (singl loc) :=
+    λ '(mk_singl ℓ) v _, ⌜ v = #ℓ ⌝%I.
+
+  Definition nil_node_prot := constant_prot (InjLV #()).
+
+  Definition cons_node_prot (x : val) (ℓtoNext : loc) :=
     λ (_ : unit) (v : val) (hG : nvmDeltaG Σ),
-      (⌜ v = (x, #ℓtoNext)%V ⌝ ∗ ϕ x hG)%I.
+      (⌜ v = (x, #ℓtoNext)%V ⌝ ∗
+       ϕ x hG)%I.
 
-  Program Instance node_inv_prot x ℓ :
-    LocationProtocol (node_inv x ℓ) := { bumper n := n }.
+  Program Instance toNext_prot_prot :
+    LocationProtocol toNext_prot := { bumper n := n }.
+  Next Obligation. Admitted.
+  Next Obligation. Admitted.
+
+  Program Instance cons_node_prot_prot x ℓ :
+    LocationProtocol (cons_node_prot x ℓ) := { bumper n := n }.
   Next Obligation.
     iIntros (?????).
-    rewrite /node_inv.
+    rewrite /cons_node_prot.
     iDestruct 1 as "[A B]".
     iCrashFlush. naive_solver.
   Qed.
   Next Obligation. iIntros. iModIntro. done. Qed.
 
   (* Representation predicate for a node. *)
-  Fixpoint is_node ℓ (xs : list val) : dProp Σ := 
+  Fixpoint is_node ℓnode (xs : list val) : dProp Σ :=
     match xs with
-    | [] => know_protocol ℓ (constant_inv (InjLV #()))
-    | x :: xs' => ∃ ℓtoNext ℓnext,
-        know_protocol ℓ (node_inv x ℓtoNext) ∗
-        know_protocol ℓnext (constant_inv #ℓ) ∗
+    | [] =>
+        ∃ q, ℓnode ↦{q} [()] ∗ know_protocol ℓnode nil_node_prot
+    | x :: xs' => ∃ ℓtoNext ℓnext q1 q2,
+        ℓnode ↦{q1} [()] ∗
+        know_protocol ℓnode (cons_node_prot x ℓtoNext) ∗
+        know_protocol ℓtoNext toNext_prot ∗
+        mapsto_na_flushed ℓtoNext q2 (mk_singl ℓnext) ∗
+        (* know_protocol ℓnext (constant_prot #ℓnode) ∗ *)
         is_node ℓnext xs'
     end.
 
   (* The invariant for the location that points to the first node in the
   stack. *)
-  Definition stack_inv (_ : unit) (v : val) (hG : nvmDeltaG Σ) : dProp Σ :=
+  Definition toHead_prot (_ : unit) (v : val) (hG : nvmDeltaG Σ) : dProp Σ :=
     ∃ (ℓnode : loc) xs,
       ⌜ v = #ℓnode ⌝ ∗
       is_node ℓnode xs ∗
       know_store_lb ℓnode () ∗
       know_flush_lb ℓnode ().
 
-  Program Instance stack_inv_prot : LocationProtocol (stack_inv) := { bumper n := n }.
+  Program Instance stack_inv_prot : LocationProtocol (toHead_prot) := { bumper n := n }.
   Next Obligation.
     iIntros (???).
-    rewrite /stack_inv.
+    rewrite /toHead_prot.
     iDestruct 1 as (??) "(A & B & stLb & flLb)".
     iCrashFlush.
     iExists ℓnode, _.
@@ -145,6 +177,39 @@ Section proof.
 
   (* The representation predicate for the entire stack. *)
   Definition is_stack (v : val) : dProp Σ :=
-    ∃ (ℓtoHead : loc), ⌜ v = #ℓtoHead ⌝ ∗ know_protocol ℓtoHead stack_inv.
+    ∃ (ℓtoHead : loc), ⌜ v = #ℓtoHead ⌝ ∗ know_protocol ℓtoHead toHead_prot.
+
+  Lemma wp_mk_stack :
+    {{{ True }}}
+      mk_stack #()
+    {{{ v, RET v; is_stack v }}} .
+  Proof.
+    iIntros (Φ) "_ ϕpost".
+    rewrite /mk_stack.
+    wp_pures.
+    wp_pures.
+    wp_bind (ref_NA _)%E.
+    iApply (wp_alloc_na _ () nil_node_prot with "[]"). { done. }
+    iNext. iIntros (ℓnil) "[#nilProt nilPts]".
+    iDestruct (mapsto_na_store_lb with "nilPts") as "#storeLb"; first done.
+    wp_pures.
+    wp_bind (WB _)%E.
+    iApply (wp_wb_lb with "[$]"). iIntros "!>". iIntros "flushLb".
+    wp_pures.
+    wp_bind Fence.
+    iApply (wp_fence with "flushLb"). iIntros "!> #flushLb".
+    wp_pures.
+
+    iApply (wp_alloc_at _ () toHead_prot with "[flushLb nilPts]"). {
+      rewrite /toHead_prot.
+      iExists _, [].
+      iSplitPure; first reflexivity.
+      iFrame "#".
+      iExists _. iFrame. }
+
+    iNext. iIntros (?) "(hi & ho & hip)".
+    iApply "ϕpost".
+    iExists _. naive_solver.
+  Qed.
 
 End proof.
